Start of effort to produce generic recursion operator for numeric terms.

examples/computability/lambda/prtermScript.sml
@@ -8,32 +8,31 @@ fun Store_thm (trip as (n,t,tac)) = store_thm trip before export_rewrites [n]
 
 val _ = new_theory "prterm"
 
-(*
-val prcons_exists = prove(
-  ``∀f n. primrec f n ⇒
-          1 < n ⇒ ∀m. ∃g. primrec g (n - 1) ∧ ∀l. g l = f (m::l)``,
-  HO_MATCH_MP_TAC strong_primrec_ind THEN SRW_TAC [][] THENL [
-    Cases_on `i` THEN SRW_TAC [][] THENL [
-      Q.EXISTS_TAC `K m` THEN SRW_TAC [ARITH_ss][],
-      Q.EXISTS_TAC `proj n'` THEN SRW_TAC [ARITH_ss][primrec_rules]
-    ],
-    FULL_SIMP_TAC (srw_ss()) [listTheory.EVERY_MEM] THEN
-    `∀m f. ∃g. MEM f gs ⇒ primrec g (n - 1) ∧ ∀l. g l = f (m::l)`
-      by METIS_TAC [] THEN
-    POP_ASSUM (Q.SPEC_THEN `m` (Q.X_CHOOSE_THEN `gf` STRIP_ASSUME_TAC o
-                                CONV_RULE SKOLEM_CONV)) THEN
-    Q.EXISTS_TAC `Cn f (MAP gf gs)` THEN
-    SRW_TAC [][] THENL [
-      MATCH_MP_TAC primrec_cn THEN
-      SRW_TAC [][listTheory.EVERY_MEM, listTheory.MEM_MAP] THEN METIS_TAC [],
-      SRW_TAC [][Cn_def, rich_listTheory.MAP_MAP_o] THEN
-      SRW_TAC [][combinTheory.o_DEF] THEN
-      AP_TERM_TAC THEN SRW_TAC [][MAP_EQ]
-    ],
-
-  *)
-
-
+val prtermrec_def = tDefine "prtermrec" `
+  prtermrec v c a list =
+    case list of
+       [] -> v []
+    || n::t ->
+        if n MOD 3 = 0 then v (n DIV 3 :: t) : num
+        else if n MOD 3 = 1 then
+          let t1 = nfst (n DIV 3) in
+          let t2 = nsnd (n DIV 3)
+          in
+            c (t1 :: t2 ::
+               prtermrec v c a (t1::t) :: prtermrec v c a (t2::t) :: t)
+        else
+          let t0 = n DIV 3
+          in
+            a (t0 :: prtermrec v c a (t0::t) :: t)`
+  (WF_REL_TAC `measure (HD o SND o SND o SND)` THEN
+   SRW_TAC [][] THEN
+   `0 < n` by (Cases_on `n` THEN FULL_SIMP_TAC (srw_ss()) []) THENL [
+     MATCH_MP_TAC LESS_EQ_LESS_TRANS THEN Q.EXISTS_TAC `n DIV 3` THEN
+     SRW_TAC [][DIV_LESS, nsnd_le],
+     MATCH_MP_TAC LESS_EQ_LESS_TRANS THEN Q.EXISTS_TAC `n DIV 3` THEN
+     SRW_TAC [][DIV_LESS, nfst_le],
+     SRW_TAC [][DIV_LESS]
+   ])
 
 val prK = prove(
   ``0 < m ⇒ primrec (λl. n) m``,
@@ -84,6 +83,342 @@ val prf2 = prove(
   STRIP_TAC THEN
   `(λl. f (g l) (h l)) = Cn (pr2 f) [g; h]` by SRW_TAC [][FUN_EQ_THM] THEN
   SRW_TAC [][primrec_rules]);
+fun i2 q = GEN_ALL (Q.INST [`f` |-> q] prf2)
+
+val prf1 = prove(
+  ``primrec g n ∧ primrec (pr1 f) 1 ⇒ primrec (λl. f (g l)) n``,
+  STRIP_TAC THEN
+  `(λl. f (g l)) = Cn (pr1 f) [g]` by SRW_TAC [][FUN_EQ_THM] THEN
+  SRW_TAC [][primrec_rules]);
+fun i1 q = GEN_ALL (Q.INST [`f` |-> q] prf1)
+
+
+val prCn1 = prove(
+  ``primrec f 1 ∧ primrec g n ⇒ primrec (λl. f [g l]) n``,
+  STRIP_TAC THEN
+  `(λl. f [g l]) = Cn f [g]` by SRW_TAC [][FUN_EQ_THM] THEN
+  SRW_TAC [][primrec_rules]);
+
+val prCn2 = prove(
+  ``primrec f 2 ∧ primrec g n ∧ primrec h n ⇒ primrec (λl. f [g l; h l]) n``,
+  STRIP_TAC THEN
+  `(λl. f [g l; h l]) = Cn f [g; h]` by SRW_TAC [][FUN_EQ_THM] THEN
+  SRW_TAC [][primrec_rules]);
+
+val prpred = prove(
+  ``pr_predicate (λl. nB (f l = g l))``,
+  SRW_TAC [][pr_predicate_def]);
+
+val NTL_def = Define`(NTL [] = []) ∧ (NTL ((h:num)::t) = t)`
+
+val strong_primrec_ind = IndDefLib.derive_strong_induction(primrec_rules,
+                                                           primrec_ind)
+
+val GENLIST_CONS = prove(
+  ``GENLIST f (SUC n) = f 0 :: (GENLIST (f o SUC) n)``,
+  Induct_on `n` THEN SRW_TAC [][GENLIST, SNOC]);
+val GENLIST1 = prove(``GENLIST f 1 = [f 0]``,
+                     SIMP_TAC bool_ss [ONE, GENLIST, SNOC]);
+val MAP_EQ_GENLIST = prove(
+  ``MAP f l = GENLIST (λi. f (EL i l)) (LENGTH l)``,
+  Induct_on `l` THEN1 SRW_TAC [][GENLIST] THEN
+  SRW_TAC [][GENLIST_CONS, combinTheory.o_DEF]);
+
+val TAKE_EQ_GENLIST = store_thm(
+  "TAKE_EQ_GENLIST",
+  ``n ≤ LENGTH l ⇒ (TAKE n l = GENLIST (λi. l ' i) n)``,
+  Q.ID_SPEC_TAC `n` THEN Induct_on `l` THEN SRW_TAC [][GENLIST] THEN
+  `∃m. n = SUC m` by (Cases_on `n` THEN SRW_TAC [][]) THEN
+  FULL_SIMP_TAC (srw_ss()) [GENLIST_CONS, combinTheory.o_DEF]);
+
+val swap2_def = Define`
+  (swap2 f [] = f [0; 0]) ∧
+  (swap2 f [n] = f [0; n]) ∧
+  (swap2 f (h1::h2::t) = f (h2::h1::t))
+`;
+
+val primrec_swap2 = store_thm(
+  "primrec_swap2",
+  ``2 ≤ n ∧ primrec f n ⇒ primrec (swap2 f) n``,
+  STRIP_TAC THEN
+  Q_TAC SUFF_TAC `swap2 f = Cn f (proj 1 :: proj 0 ::
+                                  GENLIST (λi. proj (i + 2)) (n - 2))`
+  THENL [
+    DISCH_THEN SUBST1_TAC THEN MATCH_MP_TAC primrec_cn THEN
+    SRW_TAC [ARITH_ss][LENGTH_GENLIST, primrec_rules, EVERY_GENLIST, ADD1],
+
+    SIMP_TAC (srw_ss()) [FUN_EQ_THM] THEN Q.X_GEN_TAC `l` THEN
+    `(l = []) ∨ ∃m ms. l = m::ms` by (Cases_on `l` THEN SRW_TAC [][]) THENL [
+      SRW_TAC [][Cn_def, MAP_GENLIST, combinTheory.o_DEF, swap2_def] THEN
+      Cases_on `n = 2` THEN1 SRW_TAC [][GENLIST] THEN
+      `2 < n` by DECIDE_TAC THEN
+      IMP_RES_THEN (Q.SPEC_THEN `[0; 0]` MP_TAC) primrec_short THEN
+      SRW_TAC [ARITH_ss][ADD1, combinTheory.K_DEF],
+
+      `(ms = []) ∨ ∃p ps. ms = p::ps` by (Cases_on `ms` THEN SRW_TAC [][])
+      THENL [
+        SRW_TAC [][Cn_def, MAP_GENLIST, combinTheory.o_DEF, swap2_def] THEN
+        Cases_on `n = 2` THEN1 SRW_TAC [][GENLIST] THEN
+        `2 < n` by DECIDE_TAC THEN
+        IMP_RES_THEN (Q.SPEC_THEN `[0; m]` MP_TAC) primrec_short THEN
+        SRW_TAC [ARITH_ss][ADD1, combinTheory.K_DEF],
+
+        SRW_TAC [][Cn_def, MAP_GENLIST, combinTheory.o_DEF, swap2_def] THEN
+        SRW_TAC [ARITH_ss][] THEN
+        `n ≤ LENGTH (p::m::ps) ∨ LENGTH (p::m::ps) < n` by DECIDE_TAC THENL [
+          IMP_RES_THEN (Q.SPEC_THEN `p::m::ps` MP_TAC)
+                       primrec_arg_too_long THEN
+          FULL_SIMP_TAC(srw_ss() ++ ARITH_ss) [ADD1, TAKE_EQ_GENLIST],
+
+          IMP_RES_THEN (Q.SPEC_THEN `p::m::ps` MP_TAC) primrec_short THEN
+          SRW_TAC [ARITH_ss][ADD1] THEN AP_TERM_TAC THEN SRW_TAC [][] THEN
+          FULL_SIMP_TAC (srw_ss() ++ ARITH_ss) [ADD1] THEN
+          ASM_SIMP_TAC (srw_ss() ++ ARITH_ss)
+                       [listTheory.LIST_EQ_REWRITE, LENGTH_GENLIST,
+                        EL_GENLIST] THEN
+          Q.X_GEN_TAC `i` THEN STRIP_TAC THEN
+          Cases_on `i < LENGTH ps` THEN1
+            SRW_TAC [ARITH_ss][EL_APPEND1, proj_def] THEN
+          `LENGTH ps ≤ i` by DECIDE_TAC THEN
+          SRW_TAC [ARITH_ss][EL_APPEND2, EL_GENLIST, proj_def]
+        ]
+      ]
+    ]
+  ]);
+
+val primrec_cons = store_thm(
+  "primrec_cons",
+  ``primrec f n ⇒ primrec (λl. f (c::l)) n``,
+  STRIP_TAC THEN
+  `0 < n` by IMP_RES_TAC primrec_nzero THEN
+  Q_TAC SUFF_TAC
+        `(λl. f (c::l)) = Cn f (K c :: GENLIST proj (n - 1))`
+  THENL [
+    DISCH_THEN SUBST1_TAC THEN
+    SRW_TAC [ARITH_ss][LENGTH_GENLIST, ADD1, EVERY_GENLIST, primrec_rules],
+
+    SIMP_TAC (srw_ss()) [FUN_EQ_THM] THEN Q.X_GEN_TAC `l` THEN
+    SRW_TAC [][Cn_def, MAP_GENLIST, combinTheory.o_DEF] THEN
+    `n ≤ LENGTH l + 1 ∨ LENGTH l + 1 < n` by DECIDE_TAC THENL [
+      IMP_RES_THEN (Q.SPEC_THEN `c::l` MP_TAC) primrec_arg_too_long THEN
+      SRW_TAC [ARITH_ss][ADD1, TAKE_EQ_GENLIST],
+
+      IMP_RES_THEN (Q.SPEC_THEN `c::l` MP_TAC) primrec_short THEN
+      SRW_TAC [ARITH_ss][ADD1] THEN AP_TERM_TAC THEN
+      ASM_SIMP_TAC (srw_ss() ++ ARITH_ss)
+                   [listTheory.LIST_EQ_REWRITE, LENGTH_GENLIST, EL_GENLIST]
+                   THEN
+      Q.X_GEN_TAC `i` THEN STRIP_TAC THEN
+      `i < LENGTH l ∨ LENGTH l ≤ i` by DECIDE_TAC THEN
+      SRW_TAC [ARITH_ss][proj_def, EL_APPEND1, EL_APPEND2, EL_GENLIST]
+    ]
+  ]);
+
+
+val fcons_ntl2 = store_thm(
+  "fcons_ntl2",
+  ``primrec f n ∧ primrec g (n + 2) ⇒
+    primrec (λl. f (g l :: NTL (NTL l))) (n + 2)``,
+  STRIP_TAC THEN
+  `0 < n` by METIS_TAC [primrec_nzero] THEN
+  Q.MATCH_ABBREV_TAC `primrec h (n + 2)` THEN
+  Q_TAC SUFF_TAC `h = Cn f (g::GENLIST (λi. proj (i + 2)) (n - 1))`
+  THEN1
+    (DISCH_THEN SUBST1_TAC THEN
+     MATCH_MP_TAC primrec_cn THEN
+     SRW_TAC [ARITH_ss][LENGTH_GENLIST, EVERY_GENLIST, ADD1,
+                        primrec_rules]) THEN
+  Q.UNABBREV_TAC `h` THEN SIMP_TAC (srw_ss()) [FUN_EQ_THM] THEN
+  Q.X_GEN_TAC `l` THEN SRW_TAC [][Cn_def,MAP_GENLIST, combinTheory.o_ABS_R] THEN
+  Q.PAT_ASSUM `primrec g (n + 2)` (K ALL_TAC) THEN
+  Cases_on `LENGTH (NTL (NTL l)) + 1 < n` THENL [
+    IMP_RES_THEN (Q.SPEC_THEN `g l :: NTL (NTL l)` MP_TAC) primrec_short THEN
+    SRW_TAC [ARITH_ss][ADD1] THEN AP_TERM_TAC  THEN SRW_TAC [][] THEN
+    ASM_SIMP_TAC (srw_ss() ++ ARITH_ss) [listTheory.LIST_EQ_REWRITE,
+                                         LENGTH_GENLIST, EL_GENLIST] THEN
+    Q.X_GEN_TAC `i` THEN STRIP_TAC THEN
+    Cases_on `l` THEN1 SRW_TAC [][EL_GENLIST, proj_def, NTL_def] THEN
+    SRW_TAC [ARITH_ss][NTL_def] THEN
+    Cases_on `t` THEN1 SRW_TAC [][EL_GENLIST, proj_def, NTL_def] THEN
+    SRW_TAC [ARITH_ss][NTL_def, proj_def, EL_APPEND1, EL_APPEND2,
+                       EL_GENLIST],
+
+    IMP_RES_THEN (Q.SPEC_THEN `g l :: NTL (NTL l)` MP_TAC)
+                 primrec_arg_too_long THEN
+    SRW_TAC [ARITH_ss][ADD1, TAKE_EQ_GENLIST] THEN AP_TERM_TAC THEN
+    SRW_TAC [][] THEN
+    ASM_SIMP_TAC (srw_ss() ++ ARITH_ss) [listTheory.LIST_EQ_REWRITE,
+                                         LENGTH_GENLIST, EL_GENLIST] THEN
+    Cases_on `l` THEN FULL_SIMP_TAC (srw_ss() ++ ARITH_ss) [NTL_def] THEN
+    Cases_on `t` THEN FULL_SIMP_TAC (srw_ss() ++ ARITH_ss) [NTL_def]
+  ]);
+
+
+val primrec_consNTL = store_thm(
+  "primrec_consNTL",
+  ``primrec f n ⇒ primrec (λl. f (c::NTL l)) n``,
+  STRIP_TAC THEN
+  `0 < n` by METIS_TAC [primrec_nzero] THEN
+  Q_TAC SUFF_TAC
+    `(λl. f (c::NTL l)) = Cn f (K c::GENLIST (λi. proj (i + 1)) (n - 1))`
+  THENL [
+    DISCH_THEN SUBST1_TAC THEN
+    MATCH_MP_TAC primrec_cn THEN
+    SRW_TAC [ARITH_ss][LENGTH_GENLIST, ADD1, EVERY_GENLIST, primrec_rules],
+
+    SIMP_TAC (srw_ss()) [FUN_EQ_THM] THEN Q.X_GEN_TAC `l` THEN
+    SRW_TAC [][Cn_def, MAP_GENLIST, combinTheory.o_DEF] THEN
+    `LENGTH l < n ∨ n ≤ LENGTH l` by DECIDE_TAC THENL [
+       IMP_RES_THEN (Q.SPEC_THEN `c::NTL l` MP_TAC) primrec_short THEN
+       `(l = []) ∨ ∃h t. l = h::t` by (Cases_on `l` THEN SRW_TAC [][]) THENL [
+          SRW_TAC [][NTL_def] THEN
+          `(n = 1) ∨ 1 < n` by DECIDE_TAC THEN
+          SRW_TAC [][GENLIST, combinTheory.K_DEF],
+
+          SRW_TAC [][NTL_def,ADD1] THEN
+          FULL_SIMP_TAC (srw_ss() ++ ARITH_ss) [ADD1] THEN
+          AP_TERM_TAC THEN
+          SRW_TAC [][] THEN
+          ASM_SIMP_TAC (srw_ss() ++ ARITH_ss)
+                       [listTheory.LIST_EQ_REWRITE, LENGTH_GENLIST,
+                        EL_GENLIST] THEN
+          Q.X_GEN_TAC `i` THEN STRIP_TAC THEN
+          `i < LENGTH t ∨ LENGTH t ≤ i` by DECIDE_TAC THEN
+          ASM_SIMP_TAC (srw_ss() ++ ARITH_ss)[EL_APPEND1, EL_APPEND2, proj_def,
+                                              EL_GENLIST]
+       ],
+
+       IMP_RES_THEN (Q.SPEC_THEN `c::NTL l` MP_TAC) primrec_arg_too_long THEN
+       `LENGTH (NTL l) = LENGTH l - 1`
+          by (Cases_on `l` THEN
+              FULL_SIMP_TAC (srw_ss() ++ARITH_ss) [NTL_def]) THEN
+       ASM_SIMP_TAC (srw_ss() ++ ARITH_ss) [TAKE_EQ_GENLIST] THEN
+       DISCH_THEN (K ALL_TAC) THEN
+       Cases_on `l` THEN FULL_SIMP_TAC (srw_ss() ++ ARITH_ss) [NTL_def]
+     ]
+   ]);
+
+val nlist_of_append = store_thm(
+  "nlist_of_append",
+  ``nlist_of (l1 ++ l2) = napp (nlist_of l1) (nlist_of l2)``,
+  Induct_on `l1` THEN SRW_TAC [][]);
+
+val nlist_of11 = Store_thm(
+  "nlist_of11",
+  ``∀l1 l2. (nlist_of l1 = nlist_of l2) ⇔ (l1 = l2)``,
+  Induct THEN SRW_TAC [][] THEN Cases_on `l2` THEN SRW_TAC [][]);
+
+val nlist_of_onto = store_thm(
+  "nlist_of_onto",
+  ``∀n. ∃l. nlist_of l = n``,
+  HO_MATCH_MP_TAC nlist_ind THEN SRW_TAC [][] THENL [
+    Q.EXISTS_TAC `[]` THEN SRW_TAC [][],
+    Q.EXISTS_TAC `h::l` THEN SRW_TAC [][]
+  ]);
+
+val napp_nil2 = Store_thm(
+  "napp_nil2",
+  ``∀l1. napp l1 nnil = l1``,
+  HO_MATCH_MP_TAC nlist_ind THEN SRW_TAC [][]);
+
+val napp_ASSOC = store_thm(
+  "napp_ASSOC",
+  ``napp l1 (napp l2 l3) = napp (napp l1 l2) l3``,
+  MAP_EVERY Q.ID_SPEC_TAC [`l3`, `l2`, `l1`] THEN
+  HO_MATCH_MP_TAC nlist_ind THEN SRW_TAC [][])
+
+val napp11 = Store_thm(
+  "napp11",
+  ``((napp l1 l2 = napp l1 l3) ⇔ (l2 = l3)) ∧
+    ((napp l2 l1 = napp l3 l1) ⇔ (l2 = l3))``,
+  MAP_EVERY
+      (fn (nq, lq) => Q.SPEC_THEN nq (Q.X_CHOOSE_THEN lq (SUBST1_TAC o SYM))
+                                  nlist_of_onto)
+      [(`l3`,`ll3`), (`l2`,`ll2`), (`l1`,`ll1`)] THEN
+  SRW_TAC [][GSYM nlist_of_append]);
+
+
+val prtermrec0_def = Define`
+  prtermrec0 v c a =
+   (λl. nel (l ' 0)
+            (Pr (λl. ncons (v (0::l)) nnil)
+              (λl.
+                 let n = l ' 0 + 1 in
+                 let r = l ' 1 in
+                 let m = n MOD 3 in
+                 let t = NTL (NTL l)
+                 in
+                   if m = 0 then napp r (ncons (v (n DIV 3::t)) nnil)
+                   else if m = 1 then
+                     let t1 = nfst (n DIV 3) in
+                     let t2 = nsnd (n DIV 3) in
+                     let r1 = nel t1 r in
+                     let r2 = nel t2 r
+                     in
+                       napp r (ncons (c (t1::t2::r1::r2::t)) nnil)
+                   else
+                     let t0 = n DIV 3 in
+                     let r0 = nel t0 r
+                     in
+                       napp r (ncons (a (t0::r0::t)) nnil))
+              l))`
+
+val prtermrec0_correct = store_thm(
+  "prtermrec0_correct",
+  ``prtermrec0 v c a (n::t) = prtermrec v c a (n::t)``,
+  SRW_TAC [][prtermrec0_def] THEN
+  Q.MATCH_ABBREV_TAC `nel n (f (n::t)) = prtermrec v c a (n::t)` THEN
+  Q_TAC SUFF_TAC
+    `∀n t. f (n::t) = nlist_of (GENLIST (λp. prtermrec v c a (p::t))
+                                        (n + 1))`
+    THEN1 SRW_TAC [][nel_nlist_of, LENGTH_GENLIST, EL_GENLIST] THEN
+  Induct THEN1
+    (SRW_TAC [][Abbr`f`, GENLIST1, Once prtermrec_def]) THEN
+  SRW_TAC [][Abbr`f`, LET_THM, ADD_CLAUSES, GENLIST, SNOC_APPEND,
+             nlist_of_append, NTL_def]
+  THENL [
+    SRW_TAC [ARITH_ss][Once prtermrec_def, SimpRHS, LET_THM],
+    SRW_TAC [ARITH_ss][Once prtermrec_def, SimpRHS, LET_THM] THEN
+    `nfst ((n + 1) DIV 3) < n + 1 ∧
+     nsnd ((n + 1) DIV 3) < n + 1`
+       by (CONJ_TAC THEN MATCH_MP_TAC LESS_EQ_LESS_TRANS THEN
+           Q.EXISTS_TAC `(n + 1) DIV 3` THEN
+           SRW_TAC [ARITH_ss][DIV_LESS, nsnd_le, nfst_le]) THEN
+    SRW_TAC [][nel_nlist_of, EL_GENLIST, LENGTH_GENLIST],
+    SRW_TAC [ARITH_ss][Once prtermrec_def, SimpRHS, LET_THM] THEN
+    SRW_TAC [ARITH_ss][nel_nlist_of, DIV_LESS, LENGTH_GENLIST, EL_GENLIST]
+  ]);
+
+(* val primrec_termrec = Store_thm(
+  "primrec_prtermrec",
+  ``primrec v n ∧ primrec c (n + 4) ∧ primrec a (n + 2) ⇒
+    primrec (prtermrec0 v c a) (n + 1)``,
+  SRW_TAC [][] THEN
+  `0 < n` by METIS_TAC [primrec_nzero] THEN
+  SRW_TAC [][prtermrec0_def] THEN
+  HO_MATCH_MP_TAC (i2 `nel`) THEN SRW_TAC [ARITH_ss][prproj] THEN
+  SRW_TAC [boolSimps.ETA_ss][] THEN
+  MATCH_MP_TAC alt_Pr_rule THEN SRW_TAC [ARITH_ss][] THEN1
+    (HO_MATCH_MP_TAC (i2 `ncons`) THEN SRW_TAC [][prK, primrec_cons]) THEN
+  SRW_TAC [][LET_THM] THEN
+  HO_MATCH_MP_TAC prCOND THEN SRW_TAC [][prpred, combinTheory.o_ABS_R] THENL [
+    HO_MATCH_MP_TAC (i2 `napp`) THEN SRW_TAC [ARITH_ss][prproj] THEN
+    HO_MATCH_MP_TAC (i2 `ncons`) THEN SRW_TAC [ARITH_ss][prK] THEN
+    HO_MATCH_MP_TAC fcons_ntl2 THEN
+    SRW_TAC [ARITH_ss][prDIV, prproj, i2 `$+`, prK],
+
+    HO_MATCH_MP_TAC prCOND THEN
+    SRW_TAC [][prpred, combinTheory.o_ABS_R] THENL [
+
+
+
+    SIMP_TAC (srw_ss()) [FUN_EQ_THM] THEN prtermrec_def
+
+
+
+*)
+
+
 
 val pr_is_abs_def = Define`
   pr_is_abs = (λl. nB (l ' 0 MOD 3 = 2))
@@ -103,17 +438,6 @@ val MOD3_thm = prove(
   METIS_TAC [DECIDE ``0 < 3``, arithmeticTheory.MULT_COMM,
              arithmeticTheory.MOD_EQ_0]);
 
-val prCn1 = prove(
-  ``primrec f 1 ∧ primrec g n ⇒ primrec (λl. f [g l]) n``,
-  STRIP_TAC THEN
-  `(λl. f [g l]) = Cn f [g]` by SRW_TAC [][FUN_EQ_THM] THEN
-  SRW_TAC [][primrec_rules]);
-
-val prCn2 = prove(
-  ``primrec f 2 ∧ primrec g n ∧ primrec h n ⇒ primrec (λl. f [g l; h l]) n``,
-  STRIP_TAC THEN
-  `(λl. f [g l; h l]) = Cn f [g; h]` by SRW_TAC [][FUN_EQ_THM] THEN
-  SRW_TAC [][primrec_rules]);
 
 val pr_is_abs_thm = Store_thm(
   "pr_is_abs_thm",
@@ -154,18 +478,7 @@ val pr_bnf_def = Define`
            [l ' 0; 0]))
 `;
 
-fun i2 q = GEN_ALL (Q.INST [`f` |-> q] prf2)
 
-val prf1 = prove(
-  ``primrec g n ∧ primrec (pr1 f) 1 ⇒ primrec (λl. f (g l)) n``,
-  STRIP_TAC THEN
-  `(λl. f (g l)) = Cn (pr1 f) [g]` by SRW_TAC [][FUN_EQ_THM] THEN
-  SRW_TAC [][primrec_rules]);
-fun i1 q = GEN_ALL (Q.INST [`f` |-> q] prf1)
-
-val prpred = prove(
-  ``pr_predicate (λl. nB (f l = g l))``,
-  SRW_TAC [][pr_predicate_def]);
 
 val primrec_pr_bnf = Store_thm(
   "primrec_pr_bnf",
@@ -203,44 +516,6 @@ val GENLIST_CONS = prove(
 val GENLIST1 = prove(``GENLIST f 1 = [f 0]``,
                      SIMP_TAC bool_ss [ONE, GENLIST, SNOC]);
 
-val nlist_of_append = store_thm(
-  "nlist_of_append",
-  ``nlist_of (l1 ++ l2) = napp (nlist_of l1) (nlist_of l2)``,
-  Induct_on `l1` THEN SRW_TAC [][]);
-
-val nlist_of11 = Store_thm(
-  "nlist_of11",
-  ``∀l1 l2. (nlist_of l1 = nlist_of l2) ⇔ (l1 = l2)``,
-  Induct THEN SRW_TAC [][] THEN Cases_on `l2` THEN SRW_TAC [][]);
-
-val nlist_of_onto = store_thm(
-  "nlist_of_onto",
-  ``∀n. ∃l. nlist_of l = n``,
-  HO_MATCH_MP_TAC nlist_ind THEN SRW_TAC [][] THENL [
-    Q.EXISTS_TAC `[]` THEN SRW_TAC [][],
-    Q.EXISTS_TAC `h::l` THEN SRW_TAC [][]
-  ]);
-
-val napp_nil2 = Store_thm(
-  "napp_nil2",
-  ``∀l1. napp l1 nnil = l1``,
-  HO_MATCH_MP_TAC nlist_ind THEN SRW_TAC [][]);
-
-val napp_ASSOC = store_thm(
-  "napp_ASSOC",
-  ``napp l1 (napp l2 l3) = napp (napp l1 l2) l3``,
-  MAP_EVERY Q.ID_SPEC_TAC [`l3`, `l2`, `l1`] THEN
-  HO_MATCH_MP_TAC nlist_ind THEN SRW_TAC [][])
-
-val napp11 = Store_thm(
-  "napp11",
-  ``((napp l1 l2 = napp l1 l3) ⇔ (l2 = l3)) ∧
-    ((napp l2 l1 = napp l3 l1) ⇔ (l2 = l3))``,
-  MAP_EVERY
-      (fn (nq, lq) => Q.SPEC_THEN nq (Q.X_CHOOSE_THEN lq (SUBST1_TAC o SYM))
-                                  nlist_of_onto)
-      [(`l3`,`ll3`), (`l2`,`ll2`), (`l1`,`ll1`)] THEN
-  SRW_TAC [][GSYM nlist_of_append]);
 
 val pr_bnf_correct = Store_thm(
   "pr_bnf_correct",
